src/SingleValue.v
@@ -26,8 +26,8 @@ Section System.
   Section Spec.
 
     Definition specIdx := 0.
-    Definition specChn1 := 0.
-    Definition specChn2 := 1.
+    Definition specChn1 := 1.
+    Definition specChn2 := 2.
     Definition valueIdx := 0.
 
     Definition getSpecExtIdx (idx: nat) :=
@@ -176,46 +176,20 @@ End System.
 
 Section Sim.
   Variables extIdx1 extIdx2: nat.
+  Hypotheses (Hiext1: isExternal (impl0 extIdx1 extIdx2) extIdx1 = true)
+             (Hiext2: isExternal (impl0 extIdx1 extIdx2) extIdx2 = true)
+             (Hsext1: isExternal (spec extIdx1 extIdx2) extIdx1 = true)
+             (Hsext2: isExternal (spec extIdx1 extIdx2) extIdx2 = true).
 
-  Inductive ValidValue: State -> Value -> Prop :=
-  | VVM1: forall s ost vv,
-      (st_oss s)@[child1Idx] = Some ost ->
-      ost@[statusIdx] = Some (VNat stM) ->
-      ost@[valueIdx] = Some vv ->
-      ValidValue s vv
-  | VVM2: forall s ost vv,
-      (st_oss s)@[child2Idx] = Some ost ->
-      ost@[statusIdx] = Some (VNat stM) ->
-      ost@[valueIdx] = Some vv ->
-      ValidValue s vv
-  | VVS: forall s ost1 ost2 vv,
-      (st_oss s)@[child1Idx] = Some ost1 ->
-      (st_oss s)@[child2Idx] = Some ost2 ->
-      ost1@[statusIdx] = Some (VNat stS) ->
-      ost2@[statusIdx] = Some (VNat stS) ->
-      ost1@[valueIdx] = Some vv ->
-      ost2@[valueIdx] = Some vv ->
-      ValidValue s vv.
+  Local Notation impl0 := (impl0 extIdx1 extIdx2).
+  Local Notation spec := (spec extIdx1 extIdx2).
 
-  Inductive SvmR: State -> State -> Prop :=
-  | SvmRIntro: forall ist sst st v,
-      (st_oss sst)@[specIdx] = Some st ->
-      st@[valueIdx] = Some v ->
-      ValidValue ist v ->
-      SvmR ist sst.
-
-  Theorem svm_simulation_init:
-     SvmR (getStateInit (impl0 extIdx1 extIdx2))
-          (getStateInit (spec extIdx1 extIdx2)).
-  Proof.
-    econstructor; try reflexivity.
-    eapply VVS; reflexivity.
-  Qed.
-  Hint Resolve svm_simulation_init.
+  Definition svmIdxF (idx: IdxT): IdxT :=
+    if idx ?<n (indicesOf impl0) then specIdx else idx.
 
   Definition svmMsgIdF (imid: MsgId): MsgId :=
-    {| mid_rq := mid_rq imid;
-       mid_rs := specIdx;
+    {| mid_rq := svmIdxF (mid_rq imid);
+       mid_rs := svmIdxF (mid_rs imid);
        mid_type := mid_type imid;
        mid_rqrs := mid_rqrs imid;
        mid_chn := mid_rs imid |}.
@@ -231,23 +205,165 @@ Section Sim.
     {| blbl_ins := svmMsgsF (blbl_ins b);
        blbl_outs := svmMsgsF (blbl_outs b) |}.
 
-  (* Lemma svmMsgsF_validOuts: *)
-  (*   forall from msgs, ValidOuts from msgs -> *)
-  (*                     ValidOuts from (svmMsgsF msgs). *)
-  (* Proof. *)
-  (* Admitted. *)
+  Definition SvmWf (os: StateT) v stt :=
+    os@[valueIdx] = Some v /\ os@[statusIdx] = Some stt.
 
-  Theorem svm_simulation: Simulates SvmR svmP (impl0 extIdx1 extIdx2) (spec extIdx1 extIdx2).
+  Inductive ValidValue: ObjectStates -> Value -> Prop :=
+  | VVM1: forall s ost vv,
+      s@[child1Idx] = Some ost ->
+      ost@[statusIdx] = Some (VNat stM) ->
+      ost@[valueIdx] = Some vv ->
+      ValidValue s vv
+  | VVM2: forall s ost vv,
+      s@[child2Idx] = Some ost ->
+      ost@[statusIdx] = Some (VNat stM) ->
+      ost@[valueIdx] = Some vv ->
+      ValidValue s vv
+  | VVS: forall s ost1 ost2 vv,
+      s@[child1Idx] = Some ost1 ->
+      s@[child2Idx] = Some ost2 ->
+      ost1@[statusIdx] = Some (VNat stS) ->
+      ost2@[statusIdx] = Some (VNat stS) ->
+      ost1@[valueIdx] = Some vv ->
+      ost2@[valueIdx] = Some vv ->
+      ValidValue s vv.
+
+  Inductive SvmStR: ObjectStates -> ObjectStates -> Prop :=
+  | SvmStRIntro:
+      forall ist sst sost v iost1 iost2 iostp v1 stt1 v2 stt2 vp sttp,
+        sst@[specIdx] = Some sost ->
+        sost@[valueIdx] = Some v ->
+        ist@[child1Idx] = Some iost1 ->
+        ist@[child2Idx] = Some iost2 ->
+        ist@[parentIdx] = Some iostp ->
+        SvmWf iost1 v1 stt1 ->
+        SvmWf iost2 v2 stt2 ->
+        SvmWf iostp vp sttp ->
+        ValidValue ist v ->
+        SvmStR ist sst.
+
+  Definition SvmMsgsR (imsgs smsgs: Messages) :=
+    forall to,
+      imsgs@[to] >>=[True]
+      (fun imf =>
+         forall from,
+           imf@[from] >>=[True]
+           (fun ichn =>
+              forall cidx,
+                ichn@[cidx] >>=[True]
+                (fun iq =>
+                   smsgs@[svmIdxF to] >>=[False]
+                   (fun smf =>
+                      smf@[svmIdxF from] >>=[False]
+                      (fun schn =>
+                         schn@[to] >>=[False] (fun sq => sq = svmMsgsF iq)))))).
+
+  Definition SvmR (ist sst: State) :=
+    SvmStR (st_oss ist) (st_oss sst) /\ SvmMsgsR (st_msgs ist) (st_msgs sst).
+
+  Theorem svm_simulation_init:
+     SvmR (getStateInit impl0) (getStateInit spec).
+  Proof.
+    econstructor; try (split; reflexivity).
+    econstructor; try reflexivity; try (split; reflexivity).
+    eapply VVS; reflexivity.
+  Qed.
+  Hint Resolve svm_simulation_init.
+
+  Ltac rewriter :=
+    repeat
+      match goal with
+      | [H: True |- _] => clear H
+      | [H: False |- _] => elim H
+      | [H: Some _ = Some _ |- _] => inv H
+      | [H: Some _ = None |- _] => discriminate
+      | [H: None = Some _ |- _] => discriminate
+
+      | [H: M.find ?k ?m = Some _ |- context[M.find ?k ?m] ] => rewrite H; simpl
+      | [H: M.find ?k ?m = None |- context[M.find ?k ?m] ] => rewrite H; simpl
+      | [H: Some _ = M.find ?k ?m |- context[M.find ?k ?m] ] => rewrite <-H; simpl
+      | [H: None = M.find ?k ?m |- context[M.find ?k ?m] ] => rewrite <-H; simpl
+      | [H1: M.find ?k ?m = Some _, H2: context[M.find ?k ?m] |- _] =>
+        rewrite H1 in H2; simpl in H2
+      | [H1: M.find ?k ?m = None, H2: context[M.find ?k ?m] |- _] =>
+        rewrite H1 in H2; simpl in H2
+      | [H1: Some _ = M.find ?k ?m, H2: context[M.find ?k ?m] |- _] =>
+        rewrite <-H1 in H2; simpl in H2
+      | [H1: None = M.find ?k ?m, H2: context[M.find ?k ?m] |- _] =>
+        rewrite <-H1 in H2; simpl in H2
+
+      | [H: ?te >>=[False] _ |- _] =>
+        let t := fresh "t" in
+        remember te as t; destruct t; simpl in H
+      end.
+
+  Lemma svmIdxF_extIdx1: svmIdxF extIdx1 = extIdx1.
+  Proof.
+    unfold isExternal, svmIdxF in *; destruct (extIdx1 ?<n _); [discriminate|auto].
+  Qed.
+
+  Lemma svmIdxF_extIdx2: svmIdxF extIdx2 = extIdx2.
+  Proof.
+    unfold isExternal, svmIdxF in *; destruct (extIdx2 ?<n _); [discriminate|auto].
+  Qed.
+
+  Theorem svm_simulation: Simulates SvmR svmP impl0 spec.
   Proof.
     unfold Simulates; intros.
 
     apply step_step_det in H0; inv H0.
 
-    - (* silent *) simpl; eauto.
+    - (* silent *)
+      unfold emptyLabel; rewrite toBLabel_None.
+      simpl; eauto.
 
     - (* internal *)
-      admit.
-
+      destruct H; inv H; unfold st_oss, st_msgs in *.
+      destruct sst1 as [ost1 msgs1].
+      Common.dest_in.
+      + destruct fmsg as [[frq frs fty frr fch] fval]; simpl in *.
+        inv H6; inv H7; simpl in *.
+        cbn in H1, H5; dest; subst.
+        specialize (H0 child1Idx); rewriter.
+        specialize (H0 extIdx1); apply firstMF_Some_inv in H5; dest; rewriter.
+        specialize (H0 chnImpl); apply firstC_Some_inv in H5; dest; rewriter.
+        subst.
+        destruct x0 as [|ffq fq]; [discriminate|]; simpl in H5; inv H5.
+        inv H6.
+        
+        rewrite toBLabel_Some_2 by (inv H15; rewriter; cbn; rewrite Hiext1; discriminate).
+        do 2 eexists; split.
+        * apply step_det_step.
+          eapply SsdInt; try reflexivity.
+          { left; reflexivity. }
+          { eassumption. }
+          { simpl; cbn in Heqt0; rewriter; reflexivity. }
+          { instantiate (3:= extIdx1).
+            instantiate (2:= child1Idx).
+            unfold firstMF.
+            rewrite svmIdxF_extIdx1 in Heqt1; rewrite <-Heqt1; simpl.
+            unfold firstC; rewrite <-Heqt2; simpl.
+            reflexivity.
+          }
+          { instantiate (1:= specGetReq extIdx1 extIdx2 specChn1).
+            unfold svmMsgF, svmMsgIdF; cbn.
+            rewrite svmIdxF_extIdx1.
+            reflexivity.
+          }
+          { unfold svmMsgF, svmMsgIdF; cbn.
+            repeat split; cbn.
+            apply svmIdxF_extIdx1.
+          }
+          { left; reflexivity. }
+          { simpl; auto. }
+          { simpl; reflexivity. }
+        * rewrite toBLabel_Some_2 by (cbn; rewriter; cbn; rewrite Hsext1; discriminate).
+          admit.
+          
+      + admit.
+      + admit.
+      + admit.
+        
     - (* external *)
       rewrite toBLabel_Some_1 by assumption.
       exists {| st_oss := st_oss sst1;
@@ -261,17 +377,21 @@ Section Sim.
           Common.dest_in; simpl; tauto.
         * destruct emsgs; auto.
           discriminate.
-        * admit.
-        * admit.
+        * clear -H3; induction emsgs; simpl; [apply SubList_nil|].
+          apply SubList_cons_inv in H3; dest.
+          apply SubList_cons; auto.
+          clear -H.
+          Common.dest_in;
+            destruct a as [[mrq mrs mty [|] mch] ?];
+            unfold svmMsgIdF, msgTo in *; simpl in *; subst; auto.
       + rewrite toBLabel_Some_1 by (destruct emsgs; [auto|discriminate]).
         reflexivity.
       + inv H.
         econstructor; eauto.
-        inv H6; [eapply VVM1; eauto|eapply VVM2; eauto|eapply VVS; eauto].
   Admitted.
   Hint Resolve svm_simulation.
 
-  Theorem impl0_refines_spec: (impl0 extIdx1 extIdx2) ⊑ (spec extIdx1 extIdx2).
+  Theorem impl0_refines_spec: impl0 ⊑[svmP] spec.
   Proof.
     apply simulation_implies_refinement with (sim:= SvmR); auto.
   Qed.
